refining reduction lemma in refl

pulse/examples/dsls/mini_steel/Pulse.Soundness.Exists.fsti
@@ -6,6 +6,7 @@ open Pulse.Elaborate.Pure
 open Pulse.Typing
 open Pulse.Soundness.Common
 
+module R = FStar.Reflection
 module EPure = Pulse.Elaborate.Pure
 module RT = Refl.Typing
 
@@ -30,32 +31,32 @@ val exists_inversion
 
 *)
 
-let elim_exists_post_body (u:universe) (a:term) (p:term) =
-  let erased_a = EPure.mk_erased u a in
-  let bv_0 = RT.bound_var 0 in
-  let reveal_0 = EPure.mk_reveal u a bv_0 in
-  pack_ln (Tv_App p (reveal_0, Q_Explicit))
+let elim_exists_post_body (u:universe) (a:term) (p:term) (x:var) =
+  let x_tm = var_as_term x in
+  let reveal_x = EPure.mk_reveal u a x_tm in
+  let post = pack_ln (Tv_App p (reveal_x, Q_Explicit)) in
+  RT.open_or_close_term' post (RT.CloseVar x) 0
 
-let elim_exists_post (u:universe) (a:term) (p:term) =
+let elim_exists_post (u:universe) (a:term) (p:term) (x:var) =
   let erased_a = EPure.mk_erased u a in
-  mk_abs erased_a Q_Explicit (elim_exists_post_body u a p)
+  mk_abs erased_a Q_Explicit (elim_exists_post_body u a p x)
 
 val elim_exists_soundness
-  (#f:stt_env)
-  (#g:env)
+  (#g:R.env)
   (#u:universe)
   (#a:term)
   (#p:term)
-  (a_typing:RT.typing (extend_env_l f g) a (pack_ln (Tv_Type u)))
-  (p_typing:RT.typing (extend_env_l f g) p (mk_arrow (a, Q_Explicit) vprop_tm))
-  : GTot (RT.typing (extend_env_l f g)
+  (x:var{None? (RT.lookup_bvar g x)})
+  (a_typing:RT.typing g a (pack_ln (Tv_Type u)))
+  (p_typing:RT.typing g p (mk_arrow (a, Q_Explicit) vprop_tm))
+  : GTot (RT.typing g
                  (mk_elim_exists u a p)
                  (mk_stt_ghost_comp
                     u
                     (EPure.mk_erased u a) 
                     emp_inames_tm
                     (mk_exists u a p)
-                    (elim_exists_post u a p)))
+                    (elim_exists_post u a p x)))
 
 (*
 
