pulse/examples/dsls/mini_steel/Pulse.Soundness.Exists.fst
@@ -1,6 +1,6 @@
 module Pulse.Soundness.Exists
 
 let exists_inversion _ = admit ()
-let elim_exists_soundness _ _ = admit ()
+let elim_exists_soundness _ _ _ = admit ()
 let intro_exists_soundness _ _ _ = admit ()
 let intro_exists_erased_soundness _ _ _ = admit ()
