pulse/examples/dsls/mini_steel/Pulse.Soundness.fst
@@ -282,7 +282,7 @@ let intro_exists_soundness
   Exists.intro_exists_soundness rt_typing rp_typing re_typing
 
 
-#push-options "--z3rlimit_factor 4"
+#push-options "--z3rlimit_factor 4 --fuel 2 --ifuel 2"
 let elim_exists_soundness
   (#f:stt_env)
   (#g:env)
@@ -313,36 +313,14 @@ let elim_exists_soundness
   let x_tm = Tm_Var {nm_index=x;nm_ppname=RT.pp_name_default} in
   let rx_tm = R.pack_ln (R.Tv_Var (R.pack_bv (RT.make_bv x tun))) in
   let rx_bv = R.pack_ln (R.Tv_BVar (R.pack_bv (RT.make_bv 0 tun))) in
-  assert (elab_term (mk_reveal u t x_tm) ==
-          EPure.mk_reveal ru rt rx_tm);
   calc (==) {
     elab_term (close_term' (open_term' p (mk_reveal u t x_tm) 0) x 0);
-       (==) { elab_close_commute'
-                (open_term' p (mk_reveal u t x_tm) 0)
-                x
-                0 }
-    RT.open_or_close_term' (elab_term (open_term' p (mk_reveal u t x_tm) 0)) (RT.CloseVar x) 0;
-       (==) { elab_open_commute'
-                p
-                (mk_reveal u t x_tm)
-                0 }
-    RT.open_or_close_term' (RT.open_or_close_term' rp (RT.OpenWith (EPure.mk_reveal ru rt rx_tm)) 0) (RT.CloseVar x) 0;
        (==) {
                RT.beta_reduction rt R.Q_Explicit rp (EPure.mk_reveal ru rt rx_tm)
             }
-    RT.open_or_close_term' (R.pack_ln (R.Tv_App (mk_abs rt R.Q_Explicit rp) (EPure.mk_reveal ru rt rx_tm, R.Q_Explicit))) (RT.CloseVar x) 0;
-       (==) { 
-              EPure.elab_freevars_inverse t;
-              EPure.elab_freevars_inverse p;
-              RT.close_with_not_free_var rt x 0;
-              RT.close_with_not_free_var rp x 1
-            }
-    R.pack_ln (R.Tv_App (mk_abs rt R.Q_Explicit rp)
-                        (EPure.mk_reveal ru rt rx_bv, R.Q_Explicit));
-       (==) { }
-    Exists.elim_exists_post_body ru rt (mk_abs rt R.Q_Explicit rp);
+    Exists.elim_exists_post_body ru rt (mk_abs rt R.Q_Explicit rp) x;
   };
-  Exists.elim_exists_soundness rt_typing rp_typing
+  Exists.elim_exists_soundness x rt_typing rp_typing
 #pop-options
 
 #push-options "--z3rlimit_factor 4 --query_stats"
@@ -552,19 +530,18 @@ let return_soundess
 
   elab_open_commute' post e 0;
   RT.beta_reduction rt R.Q_Explicit (elab_term post) re;
-  RT.beta_reduction_bv0 rt R.Q_Explicit (elab_term post);
   
   match ctag, use_eq with
   | STT, true ->
-    Return.return_stt_typing rt_typing re_typing rpost_typing
+    Return.return_stt_typing x rt_typing re_typing rpost_typing
   | STT, false -> 
     Return.return_stt_noeq_typing rt_typing re_typing rpost_typing
   | STT_Atomic, true ->
-    Return.return_stt_atomic_typing rt_typing re_typing rpost_typing
+    Return.return_stt_atomic_typing x rt_typing re_typing rpost_typing
   | STT_Atomic, false -> 
     Return.return_stt_atomic_noeq_typing rt_typing re_typing rpost_typing
   | STT_Ghost, true ->
-    Return.return_stt_ghost_typing rt_typing re_typing rpost_typing
+    Return.return_stt_ghost_typing x rt_typing re_typing rpost_typing
   | STT_Ghost, false -> 
     Return.return_stt_ghost_noeq_typing rt_typing re_typing rpost_typing
 
